src/Init/System/IOError.lean
@@ -8,7 +8,7 @@ module
 
 prelude
 public import Init.Data.ToString.Basic
-import Init.Data.String.Basic
+import Init.Data.String.Modify
 
 public section
 
