src/Lean/ErrorExplanation.lean
@@ -11,6 +11,7 @@ public import Lean.Message
 public import Lean.EnvExtension
 public import Lean.DocString.Links
 import Init.Data.String.TakeDrop
+import Init.Data.String.Extra
 
 public section
 
