src/Std/Time/Format/Basic.lean
@@ -8,6 +8,7 @@ module
 prelude
 public import Std.Time.Zoned
 import Init.Data.String.TakeDrop
+import Init.Data.String.Extra
 
 public section
 
