src/lake/Lake/Build/Trace.lean
@@ -10,6 +10,7 @@ public import Lean.Data.Json
 import Init.Data.Nat.Fold
 import Lake.Util.String
 import Lake.Util.IO
+public import Init.Data.String.Extra
 
 /-! # Lake Traces
 
